
Introduction:
Hello and welcome to this tutorial on the Laws of Exponents. In this video, we'll be covering nine important rules that are fundamental to understanding and working with exponents.

Rule 1: One Exponent Rule
The first rule we'll be discussing is the One Exponent Rule. This rule states that any number raised to the power of 1 is equal to the number itself. For example, 5^1 = 5, and 10^1 = 10. Here are five more examples:

1. 3^1 = 3
2. 9^1 = 9
3. 2^1 = 2
4. 11^1 = 11
5. 0.5^1 = 0.5

Rule 2: Zero Exponent Rule
The Zero Exponent Rule tells us that any number raised to the power of 0 is equal to 1. For example, 3^0 = 1 and 10^0 = 1. Here are five more examples:

1. 7^0 = 1
2. 0.2^0 = 1
3. 100^0 = 1
4. 2^0 = 1
5. 11^0 = 1

Rule 3: Negative Exponent Rule
The Negative Exponent Rule states that if a number is raised to a negative power, we can rewrite it as 1 divided by the number raised to the positive version of that power. For example, 2^-3 can be rewritten as 1/2^3. Here are five more examples:

1. 5^-2 = 1/5^2
2. 8^-4 = 1/8^4
3. 0.1^-1 = 1/0.1^1
4. 3^-5 = 1/3^5
5. 2^-6 = 1/2^6

Rule 4: Product Exponent Rule
The Product Exponent Rule tells us that when multiplying two numbers with the same base, we can add their exponents together. For example, 4^2 x 4^3 = 4^(2+3) = 4^5. Here are five more examples:

1. 2^4 x 2^6 = 2^(4+6) = 2^10
2. 9^2 x 9^5 = 9^(2+5) = 9^7
3. 5^3 x 5^9 = 5^(3+9) = 5^12
4. 11^6 x 11^2 = 11^(6+2) = 11^8
5. 0.1^2 x 0.1^5 = 0.1^(2+5) = 0.1^7

Rule 5: Quotient Exponent Rule (continued)
The Quotient Exponent Rule tells us that when a number is divided by another number and both numbers are raised to the same exponent, we can simplify the expression by subtracting the exponents. For example, (3^4)/(3^2) = 3^(4-2) = 3^2 = 9. Here are five more examples:

(2^6)/(2^2) = 2^(6-2) = 2^4 = 16
(5^8)/(5^4) = 5^(8-4) = 5^4 = 625
(7^3)/(7^2) = 7^(3-2) = 7^1 = 7
(4^5)/(4^3) = 4^(5-3) = 4^2 = 16
(9^4)/(9^3) = 9^(4-3) = 9^1 = 9

Rule 6: Power of a Power Rule
The Power of a Power Rule tells us that when a number is raised to a power and then that result is raised to another power, we can multiply the exponents together. For example, (2^3)^2 = 2^(3x2) = 2^6. Here are five more examples:

1. (3^2)^3 = 3^(2x3) = 3^6
2. (10^3)^2 = 10^(3x2) = 10^6
3. (5^4)^3 = 5^(4x3) = 5^12
4. (8^2)^4 = 8^(2x4) = 8^8
5. (0.5^3)^2 = 0.5^(3x2) = 0.5^6

Rule 7: Power of a Product Rule
The Power of a Product Rule tells us that when a product of numbers is raised to a power, we can distribute that power to each number in the product. For example, (4 x 3)^2 = 4^2 x 3^2 = 16 x 9. Here are five more examples:

1. (5 x 2)^3 = 5^3 x 2^3 = 125 x 8
2. (9 x 6)^2 = 9^2 x 6^2 = 81 x 36
3. (2 x 3 x 4)^3 = 2^3 x 3^3 x 4^3 = 8 x 27 x 64
4. (7 x 8 x 9)^2 = 7^2 x 8^2 x 9^2 = 49 x 64 x 81
5. (0.1 x 0.2)^3 = 0.1^3 x 0.2^3 = 0.001 x 0.008

Rule 8: Power of a Quotient Rule
The Power of a Quotient Rule tells us that when a quotient of numbers is raised to a power, we can distribute that power to each number in the quotient. For example, (16/2)^3 = 16^3 / 2^3 = 4096. Here are five more examples:

1. (25/5)^2 = 25^2 / 5^2 = 625 / 25 = 25
2. (27/3)^4 = 27^4 / 3^4 = 531441 / 81 = 6561
3. (12/2)^5 = 12^5 / 2^5 = 248832 / 32 = 7776
4. (0.5/0.1)^3 = 0.5^3 / 0.1^3 = 0.125 / 0.001 = 125
5. (36/6)^2 = 36^2 / 6^2 = 1296 / 36 = 36

Rule 9: Rational Exponent Rule (continued)
The Rational Exponent Rule is used when a number is raised to a fractional power. To apply this rule, we can rewrite the number as a radical and simplify. For example, 16^(1/2) = sqrt(16) = 4. Here are five more examples:

1. 27^(1/3) = cuberoot(27) = 3
2. 64^(2/3) = (64^(1/3))^2 = 4^2 = 16
3. 125^(2/3) = (125^(1/3))^2 = 5^2 = 25
4. 8^(3/4) = (8^(1/4))^3 = 2^3 = 8
5. 16^(3/2) = (16^(1/2))^3 = 4^3 = 64

Conclusion:
And that's it for our tutorial on the Laws of Exponents! By understanding and applying these rules, you'll be able to simplify and solve complex exponent expressions with ease. Thanks for watching, and see you in the next video!
